dist/linux/Hacl_Curve25519_51.c
@@ -63,7 +63,7 @@ inline void Hacl_Impl_Curve25519_Field51_fsub(u64 *out, u64 *f1, u64 *f2)
 }
 
 inline void
-Hacl_Impl_Curve25519_Field51_fmul(u64 *out, u64 *f1, u64 *f2, uint128_t *uu____2959)
+Hacl_Impl_Curve25519_Field51_fmul(u64 *out, u64 *f1, u64 *f2, uint128_t *uu____3153)
 {
   u64 f10 = f1[0U];
   u64 f11 = f1[1U];
@@ -339,7 +339,7 @@ inline void Hacl_Impl_Curve25519_Field51_fmul1(u64 *out, u64 *f1, u64 f2)
   out[4U] = o4;
 }
 
-inline void Hacl_Impl_Curve25519_Field51_fsqr(u64 *out, u64 *f, uint128_t *uu____6941)
+inline void Hacl_Impl_Curve25519_Field51_fsqr(u64 *out, u64 *f, uint128_t *uu____7683)
 {
   u64 f0 = f[0U];
   u64 f1 = f[1U];
