code/hash/Hacl.Impl.SHA2.Core.fsti
@@ -15,3 +15,18 @@ val sha256: hash:lbuffer uint8 32ul -> len:size_t -> b:buffer uint8{length b == 
     (requires (fun h0 -> live h0 b /\ live h0 hash /\ disjoint hash b))
     (ensures (fun h0 _ h1 -> modifies (loc hash) h0 h1))
 
+val sha256_4: r0:lbuffer uint8 32ul ->
+              r1:lbuffer uint8 32ul ->
+              r2:lbuffer uint8 32ul ->
+              r3:lbuffer uint8 32ul ->
+              len:size_t ->
+              b0:buffer uint8{length b0 == v len} ->
+              b1:buffer uint8{length b1 == v len} ->
+              b2:buffer uint8{length b2 == v len} ->
+              b3:buffer uint8{length b3 == v len} ->
+    Stack unit
+    (requires (fun h0 -> live h0 b0 /\ live h0 b1 /\ live h0 b2 /\ live h0 b3 /\ 
+                       live h0 r0 /\ live h0 r1 /\ live h0 r2 /\ live h0 r3))
+    (ensures (fun h0 _ h1 -> modifies (loc r0 |+| loc r1 |+| loc r2 |+| loc r3) h0 h1))
+
+
